modernized specifications; tuned proofs;

thys/MiniML/Instance.thy
@@ -1,5 +1,5 @@
 (* Title:     HOL/MiniML/Instance.thy
-   ID:        $Id: Instance.thy,v 1.6 2004-08-18 07:24:54 nipkow Exp $
+   ID:        $Id: Instance.thy,v 1.7 2007-10-03 19:09:51 makarius Exp $
    Author:    Wolfgang Naraschewski and Tobias Nipkow
    Copyright  1996 TU Muenchen
 *)
@@ -26,62 +26,46 @@ primrec
   "bound_scheme_inst S (BVar n) = (S n)"
   "bound_scheme_inst S (sch1 =-> sch2) = ((bound_scheme_inst S sch1) =-> (bound_scheme_inst S sch2))"
   
-consts
-  "<|" :: "[typ, type_scheme] => bool" (infixr 70)
-defs
-  is_bound_typ_instance: "t <| sch == ? S. t = (bound_typ_inst S sch)" 
+definition
+  is_bound_typ_instance :: "[typ, type_scheme] => bool"  (infixr "<|" 70) where
+  is_bound_typ_instance: "t <| sch = (? S. t = (bound_typ_inst S sch))"
 
 instance type_scheme :: ord ..
-defs le_type_scheme_def: "sch' <= (sch::type_scheme) == !t. t <| sch' --> t <| sch"
+defs (overloaded)
+  le_type_scheme_def: "sch' <= (sch::type_scheme) == !t. t <| sch' --> t <| sch"
 
 consts
   subst_to_scheme :: "[nat => type_scheme, typ] => type_scheme"
-
 primrec
   "subst_to_scheme B (TVar n) = (B n)"
   "subst_to_scheme B (t1 -> t2) = ((subst_to_scheme B t1) =-> (subst_to_scheme B t2))"
   
 instance list :: (ord)ord ..
-defs le_env_def:
-  "A <= B == length B = length A & (!i. i < length A --> A!i <= B!i)"
+defs (overloaded)
+  le_env_def: "A <= B == length B = length A & (!i. i < length A --> A!i <= B!i)"
 
 
 text "lemmas for instatiation"
 
-lemma bound_typ_inst_mk_scheme: "bound_typ_inst S (mk_scheme t) = t"
-apply (induct_tac "t")
-apply (simp_all (no_asm_simp))
-done
+lemma bound_typ_inst_mk_scheme [simp]: "bound_typ_inst S (mk_scheme t) = t"
+  by (induct t) simp_all
 
-declare bound_typ_inst_mk_scheme [simp]
+lemma bound_typ_inst_composed_subst [simp]:
+    "bound_typ_inst ($S o R) ($S sch) = $S (bound_typ_inst R sch)"
+  by (induct sch) simp_all
 
-lemma bound_typ_inst_composed_subst: "bound_typ_inst ($S o R) ($S sch) = $S (bound_typ_inst R sch)"
-apply (induct_tac "sch")
-apply simp_all
-done
+lemma bound_typ_inst_eq:
+    "S = S' ==> sch = sch' ==> bound_typ_inst S sch = bound_typ_inst S' sch'"
+  by simp
 
-declare bound_typ_inst_composed_subst [simp]
-
-lemma bound_typ_inst_eq: "S = S' ==> sch = sch' ==> bound_typ_inst S sch = bound_typ_inst S' sch'"
-apply simp
-done
-
-lemma bound_scheme_inst_mk_scheme: "bound_scheme_inst B (mk_scheme t) = mk_scheme t"
-apply (induct_tac "t")
-apply (simp (no_asm))
-apply (simp (no_asm_simp))
-done
-
-declare bound_scheme_inst_mk_scheme [simp]
+lemma bound_scheme_inst_mk_scheme [simp]:
+    "bound_scheme_inst B (mk_scheme t) = mk_scheme t"
+  by (induct t) simp_all
 
 lemma substitution_lemma: "$S (bound_scheme_inst B sch) = (bound_scheme_inst ($S o B) ($ S sch))"
-apply (induct_tac "sch")
-apply (simp (no_asm))
-apply (simp (no_asm))
-apply (simp (no_asm_simp))
-done
+  by (induct sch) simp_all
 
-lemma bound_scheme_inst_type [rule_format (no_asm)]: "!t. mk_scheme t = bound_scheme_inst B sch -->  
+lemma bound_scheme_inst_type [rule_format]: "!t. mk_scheme t = bound_scheme_inst B sch -->  
           (? S. !x:bound_tv sch. B x = mk_scheme (S x))"
 apply (induct_tac "sch")
 apply (simp (no_asm))
@@ -103,33 +87,29 @@ apply (rule_tac x = "%x. if x:bound_tv type_scheme1 then (S1 x) else (S2 x) " in
 apply auto
 done
 
-lemma subst_to_scheme_inverse [rule_format (no_asm)]: 
-  "new_tv n sch --> 
-  subst_to_scheme (%k. if n <= k then BVar (k - n) else FVar k)  
-                  (bound_typ_inst (%k. TVar (k + n)) sch) = sch"
-apply (induct_tac "sch")
-apply (simp (no_asm) add: le_def)
-apply (simp (no_asm) add: le_add2 diff_add_inverse2)
-apply (simp (no_asm_simp))
-done
+lemma subst_to_scheme_inverse: 
+  "new_tv n sch \<Longrightarrow>
+    subst_to_scheme (%k. if n <= k then BVar (k - n) else FVar k)  
+      (bound_typ_inst (%k. TVar (k + n)) sch) = sch"
+  apply (induct sch)
+    apply (simp add: le_def)
+   apply (simp add: le_add2 diff_add_inverse2)
+  apply simp
+  done
 
 lemma aux: "t = t' ==>  
       subst_to_scheme (%k. if n <= k then BVar (k - n) else FVar k) t =  
       subst_to_scheme (%k. if n <= k then BVar (k - n) else FVar k) t'"
-apply fast
-done
+  by blast
 
-lemma aux2 [rule_format]: "new_tv n sch -->  
-      subst_to_scheme (%k. if n <= k then BVar (k - n) else FVar k) (bound_typ_inst S sch) =  
-       bound_scheme_inst ((subst_to_scheme (%k. if n <= k then BVar (k - n) else FVar k)) o S) sch"
-apply (induct_tac "sch")
-apply auto
-done
+lemma aux2: "new_tv n sch \<Longrightarrow>
+  subst_to_scheme (%k. if n <= k then BVar (k - n) else FVar k) (bound_typ_inst S sch) =  
+    bound_scheme_inst ((subst_to_scheme (%k. if n <= k then BVar (k - n) else FVar k)) o S) sch"
+    by (induct sch) auto
 
-lemma le_type_scheme_def2: 
-  "!!(sch::type_scheme) sch'.  
-   (sch' <= sch) = (? B. sch' = bound_scheme_inst B sch)"
-
+lemma le_type_scheme_def2:
+  fixes sch sch' :: type_scheme
+  shows "(sch' <= sch) = (? B. sch' = bound_scheme_inst B sch)"
 apply (unfold le_type_scheme_def is_bound_typ_instance)
 apply (rule iffI)
 apply (cut_tac sch = "sch" in fresh_variable_type_schemes)
@@ -156,7 +136,7 @@ apply (simp (no_asm))
 apply (simp (no_asm_simp))
 done
 
-lemma le_type_eq_is_bound_typ_instance [rule_format (no_asm)]: "(mk_scheme t) <= sch = t <| sch"
+lemma le_type_eq_is_bound_typ_instance [rule_format]: "(mk_scheme t) <= sch = t <| sch"
 apply (unfold is_bound_typ_instance)
 apply (simp (no_asm) add: le_type_scheme_def2)
 apply (rule iffI)
@@ -184,7 +164,7 @@ apply (simp (no_asm))
 apply simp
 done
 
-lemma le_env_Cons: 
+lemma le_env_Cons [iff]: 
   "(sch # A <= sch' # B) = (sch <= (sch'::type_scheme) & A <= B)"
 apply (unfold le_env_def)
 apply (simp (no_asm))
@@ -201,20 +181,21 @@ apply (rule conjI)
  apply fast
 apply (rule allI)
 apply (induct_tac "i")
-apply (simp_all (no_asm_simp))
+apply simp_all
 done
-declare le_env_Cons [iff]
 
 lemma is_bound_typ_instance_closed_subst: "t <| sch ==> $S t <| $S sch"
 apply (unfold is_bound_typ_instance)
 apply (erule exE)
 apply (rename_tac "SA") 
-apply (simp)
+apply simp
 apply (rule_tac x = "$S o SA" in exI)
-apply (simp (no_asm))
+apply simp
 done
 
-lemma S_compatible_le_scheme: "!!(sch::type_scheme) sch'. sch' <= sch ==> $S sch' <= $ S sch"
+lemma S_compatible_le_scheme:
+  fixes sch sch' :: type_scheme
+  shows "sch' <= sch ==> $S sch' <= $ S sch"
 apply (simp add: le_type_scheme_def2)
 apply (erule exE)
 apply (simp add: substitution_lemma)
@@ -222,78 +203,54 @@ apply fast
 done
 
 lemma S_compatible_le_scheme_lists: 
- "!!(A::type_scheme list) A'. A' <= A ==> $S A' <= $ S A"
+  fixes A A' :: "type_scheme list"
+  shows "A' <= A ==> $S A' <= $ S A"
 apply (unfold le_env_def app_subst_list)
-apply (simp (no_asm) cong add: conj_cong)
+apply (simp cong add: conj_cong)
 apply (fast intro!: S_compatible_le_scheme)
 done
 
 lemma bound_typ_instance_trans: "[| t <| sch; sch <= sch' |] ==> t <| sch'"
-apply (unfold le_type_scheme_def)
-apply fast
-done
+  unfolding le_type_scheme_def by blast
 
-lemma le_type_scheme_refl: "sch <= (sch::type_scheme)"
-apply (unfold le_type_scheme_def)
-apply fast
-done
-declare le_type_scheme_refl [iff]
+lemma le_type_scheme_refl [iff]: "sch <= (sch::type_scheme)"
+  unfolding le_type_scheme_def by blast
 
-lemma le_env_refl: "A <= (A::type_scheme list)"
-apply (unfold le_env_def)
-apply fast
-done
-declare le_env_refl [iff]
+lemma le_env_refl [iff]: "A <= (A::type_scheme list)"
+  unfolding le_env_def by blast
 
-lemma bound_typ_instance_BVar: "sch <= BVar n"
+lemma bound_typ_instance_BVar [iff]: "sch <= BVar n"
 apply (unfold le_type_scheme_def is_bound_typ_instance)
 apply (intro strip)
 apply (rule_tac x = "%a. t" in exI)
-apply (simp (no_asm))
+apply simp
 done
-declare bound_typ_instance_BVar [iff]
 
-lemma le_FVar: 
- "(sch <= FVar n) = (sch = FVar n)"
+lemma le_FVar [simp]: "(sch <= FVar n) = (sch = FVar n)"
 apply (unfold le_type_scheme_def is_bound_typ_instance)
 apply (induct_tac "sch")
-  apply (simp (no_asm))
- apply (simp (no_asm))
- apply fast
+apply auto
+done
+
+lemma not_FVar_le_Fun [iff]: "~(FVar n <= sch1 =-> sch2)"
+  unfolding le_type_scheme_def is_bound_typ_instance by simp
+
+lemma not_BVar_le_Fun [iff]: "~(BVar n <= sch1 =-> sch2)"
+apply (unfold le_type_scheme_def is_bound_typ_instance)
 apply simp
-apply fast
-done
-declare le_FVar [simp]
-
-lemma not_FVar_le_Fun: "~(FVar n <= sch1 =-> sch2)"
-apply (unfold le_type_scheme_def is_bound_typ_instance)
-apply (simp (no_asm))
-done
-declare not_FVar_le_Fun [iff]
-
-lemma not_BVar_le_Fun: "~(BVar n <= sch1 =-> sch2)"
-apply (unfold le_type_scheme_def is_bound_typ_instance)
-apply (simp (no_asm))
 apply (rule_tac x = "TVar n" in exI)
-apply (simp (no_asm))
-apply fast
+apply fastsimp
 done
-declare not_BVar_le_Fun [iff]
 
 lemma Fun_le_FunD: 
   "(sch1 =-> sch2 <= sch1' =-> sch2') ==> sch1 <= sch1' & sch2 <= sch2'"
-apply (unfold le_type_scheme_def is_bound_typ_instance)
-apply (fastsimp)
-done
+  unfolding le_type_scheme_def is_bound_typ_instance by fastsimp
 
-lemma scheme_le_Fun [rule_format (no_asm)]: "(sch' <= sch1 =-> sch2) --> (? sch'1 sch'2. sch' = sch'1 =-> sch'2)"
-apply (induct_tac "sch'")
-apply (simp (no_asm_simp))
-apply (simp (no_asm_simp))
-apply fast
-done
+lemma scheme_le_Fun: "(sch' <= sch1 =-> sch2) \<Longrightarrow> ? sch'1 sch'2. sch' = sch'1 =-> sch'2"
+  by (induct sch') auto
 
-lemma le_type_scheme_free_tv [rule_format (no_asm)]: "!sch'::type_scheme. sch <= sch' --> free_tv sch' <= free_tv sch"
+lemma le_type_scheme_free_tv [rule_format]:
+  "!sch'::type_scheme. sch <= sch' --> free_tv sch' <= free_tv sch"
 apply (induct_tac "sch")
   apply (rule allI)
   apply (induct_tac "sch'")
@@ -315,7 +272,8 @@ apply (drule Fun_le_FunD)
 apply fast
 done
 
-lemma le_env_free_tv [rule_format (no_asm)]: "!A::type_scheme list. A <= B --> free_tv B <= free_tv A"
+lemma le_env_free_tv [rule_format]:
+  "!A::type_scheme list. A <= B --> free_tv B <= free_tv A"
 apply (induct_tac "B")
  apply (simp (no_asm))
 apply (rule allI)
