thys/MiniML/Type.thy
@@ -1,5 +1,5 @@
 (* Title:     HOL/MiniML/Type.thy
-   ID:        $Id: Type.thy,v 1.11 2007-09-28 13:15:24 lp15 Exp $
+   ID:        $Id: Type.thy,v 1.12 2007-10-03 19:09:51 makarius Exp $
    Author:    Wolfgang Naraschewski and Tobias Nipkow
    Copyright  1996 TU Muenchen
 *)
@@ -14,15 +14,14 @@ begin
 axclass  type_struct < type
 
 -- "type expressions"
-datatype "typ" = TVar nat | "->" "typ" "typ" (infixr 70)
+datatype "typ" = TVar nat | Fun "typ" "typ" (infixr "->" 70)
 
 -- "type schemata"
-datatype type_scheme = FVar nat | BVar nat | "=->" type_scheme type_scheme (infixr 70)
+datatype type_scheme = FVar nat | BVar nat | SFun type_scheme type_scheme (infixr "=->" 70)
 
 -- "embedding types into type schemata"
 consts
   mk_scheme :: "typ => type_scheme"
-
 primrec
   "mk_scheme (TVar n) = (FVar n)"
   "mk_scheme (t1 -> t2) = ((mk_scheme t1) =-> (mk_scheme t2))"
@@ -121,7 +120,7 @@ primrec (app_subst_type_scheme)
   "$ S (BVar n) = (BVar n)"
   "$ S (sch1 =-> sch2) = ($ S sch1) =-> ($ S sch2)"
 
-defs
+defs (overloaded)
   app_subst_list: "$ S == map ($ S)"
 
 -- "domain of a substitution"
@@ -134,7 +133,7 @@ definition
   cod :: "subst => nat set" where
   "cod S = (UN m:dom S. (free_tv (S m)))"
 
-defs
+defs (overloaded)
   free_tv_subst: "free_tv S == (dom S) Un (cod S)" 
 
   
@@ -150,14 +149,14 @@ axioms
 
 declare mgu_eq [simp] mgu_mg [simp] mgu_free [simp]
 
-lemma mk_scheme_Fun [rule_format (no_asm)]: "mk_scheme t = sch1 =-> sch2 --> (? t1 t2. sch1 = mk_scheme t1 & sch2 = mk_scheme t2)"
+lemma mk_scheme_Fun [rule_format]: "mk_scheme t = sch1 =-> sch2 --> (? t1 t2. sch1 = mk_scheme t1 & sch2 = mk_scheme t2)"
 apply (induct_tac "t")
 apply (simp (no_asm))
 apply simp
 apply fast
 done
 
-lemma mk_scheme_injective [rule_format (no_asm)]: "!t'. mk_scheme t = mk_scheme t' --> t=t'"
+lemma mk_scheme_injective [rule_format]: "!t'. mk_scheme t = mk_scheme t' --> t=t'"
 apply (induct_tac "t")
  apply (rule allI)
  apply (induct_tac "t'")
@@ -258,57 +257,32 @@ declare
   new_tv_Fun [simp] new_tv_Fun2 [simp] new_tv_Nil [simp] 
   new_tv_Cons [simp] new_tv_TVar_subst [simp]
 
-lemma new_tv_id_subst: 
-  "new_tv n id_subst"
-apply (unfold id_subst_def new_tv_def free_tv_subst dom_def cod_def)
-apply (simp (no_asm))
-done
-declare new_tv_id_subst [simp]
+lemma new_tv_id_subst [simp]: "new_tv n id_subst"
+  by (simp add: id_subst_def new_tv_def free_tv_subst dom_def cod_def)
 
-lemma new_if_subst_type_scheme: "new_tv n (sch::type_scheme) -->  
-      $(%k. if k<n then S k else S' k) sch = $S sch"
-apply (induct_tac "sch")
-apply (simp_all (no_asm_simp))
-done
-declare new_if_subst_type_scheme [simp]
+lemma new_if_subst_type_scheme [simp]: "new_tv n (sch::type_scheme) \<Longrightarrow>
+    $(%k. if k<n then S k else S' k) sch = $S sch"
+  by (induct sch) simp_all
 
-lemma new_if_subst_type_scheme_list: "new_tv n (A::type_scheme list) -->  
-      $(%k. if k<n then S k else S' k) A = $S A"
-apply (induct_tac "A")
-apply (simp_all (no_asm_simp))
-done
-declare new_if_subst_type_scheme_list [simp]
+lemma new_if_subst_type_scheme_list [simp]: "new_tv n (A::type_scheme list) \<Longrightarrow>
+    $(%k. if k<n then S k else S' k) A = $S A"
+  by (induct A) simp_all
 
 
 -- "constructor laws for @{text dom} and @{text cod}"
 
-lemma dom_id_subst: 
-  "dom id_subst = {}"
+lemma dom_id_subst [simp]: "dom id_subst = {}"
+  unfolding dom_def id_subst_def empty_def by simp
 
-apply (unfold dom_def id_subst_def empty_def)
-apply (simp (no_asm))
-done
-declare dom_id_subst [simp]
-
-lemma cod_id_subst: 
-  "cod id_subst = {}"
-apply (unfold cod_def)
-apply (simp (no_asm))
-done
-declare cod_id_subst [simp]
+lemma cod_id_subst [simp]: "cod id_subst = {}"
+  unfolding cod_def by simp
 
 
--- "lemmata for @{text free_tv}"
+lemma free_tv_id_subst [simp]: "free_tv id_subst = {}"
+  unfolding free_tv_subst by simp
 
-lemma free_tv_id_subst: 
-  "free_tv id_subst = {}"
-
-apply (unfold free_tv_subst)
-apply (simp (no_asm))
-done
-declare free_tv_id_subst [simp]
-
-lemma free_tv_nth_A_impl_free_tv_A [rule_format (no_asm)]: "!n. n < length A --> x : free_tv (A!n) --> x : free_tv A"
+lemma free_tv_nth_A_impl_free_tv_A [rule_format, simp]:
+  "!n. n < length A --> x : free_tv (A!n) --> x : free_tv A"
 apply (induct_tac "A")
 apply simp
 apply (rule allI)
@@ -317,9 +291,7 @@ apply simp
 apply simp
 done
 
-declare free_tv_nth_A_impl_free_tv_A [simp]
-
-lemma free_tv_nth_nat_A [rule_format (no_asm)]: 
+lemma free_tv_nth_nat_A [rule_format]:
   "!nat. nat < length A --> x : free_tv (A!nat) --> x : free_tv A"
 apply (induct_tac "A")
 apply simp
@@ -327,7 +299,7 @@ apply (rule allI)
 apply (induct_tac "nat" rule: nat_induct)
 apply (intro strip)
 apply simp
-apply (simp (no_asm))
+apply simp
 done
 
 text
@@ -335,105 +307,83 @@ text
    structure the substitutions coincide on the free type variables
    occurring in the type structure *}
 
-lemma typ_substitutions_only_on_free_variables [rule_format (no_asm)]: 
-  "(!x:free_tv t. (S x) = (S' x)) --> $ S (t::typ) = $ S' t"
-apply (induct_tac "t")
-apply (simp (no_asm))
-apply simp
-done
+lemma typ_substitutions_only_on_free_variables: 
+  "(!x:free_tv t. (S x) = (S' x)) \<Longrightarrow> $ S (t::typ) = $ S' t"
+  by (induct t) simp_all
 
 lemma eq_free_eq_subst_te: "(!n. n:(free_tv t) --> S1 n = S2 n) ==> $ S1 (t::typ) = $ S2 t"
 apply (rule typ_substitutions_only_on_free_variables)
-apply (simp (no_asm) add: Ball_def)
-done
-
-lemma scheme_substitutions_only_on_free_variables [rule_format (no_asm)]: 
-  "(!x:free_tv sch. (S x) = (S' x)) --> $ S (sch::type_scheme) = $ S' sch"
-apply (induct_tac "sch")
-apply (simp (no_asm))
-apply (simp (no_asm))
 apply simp
 done
+
+lemma scheme_substitutions_only_on_free_variables:
+  "(!x:free_tv sch. (S x) = (S' x)) \<Longrightarrow> $ S (sch::type_scheme) = $ S' sch"
+  by (induct sch) simp_all
 
 lemma eq_free_eq_subst_type_scheme: 
   "(!n. n:(free_tv sch) --> S1 n = S2 n) ==> $ S1 (sch::type_scheme) = $ S2 sch"
 apply (rule scheme_substitutions_only_on_free_variables)
-apply (simp (no_asm) add: Ball_def)
+apply simp
 done
 
-lemma eq_free_eq_subst_scheme_list [rule_format (no_asm)]: 
-  "(!n. n:(free_tv A) --> S1 n = S2 n) --> $S1 (A::type_scheme list) = $S2 A"
-apply (induct_tac "A")
-(* case [] *)
-apply (fastsimp)
-(* case x#xl *)
-apply (fastsimp intro: eq_free_eq_subst_type_scheme)
-done
+lemma eq_free_eq_subst_scheme_list:
+  "(!n. n:(free_tv A) --> S1 n = S2 n) \<Longrightarrow> $S1 (A::type_scheme list) = $S2 A"
+proof (induct A)
+  case Nil then show ?case by fastsimp
+next
+  case Cons then show ?case by (fastsimp intro: eq_free_eq_subst_type_scheme)
+qed
 
 lemma weaken_asm_Un: "((!x:A. (P x)) --> Q) ==> ((!x:A Un B. (P x)) --> Q)"
-apply fast
-done
+  by fast
 
-lemma scheme_list_substitutions_only_on_free_variables [rule_format (no_asm)]: "(!x:free_tv A. (S x) = (S' x)) --> $ S (A::type_scheme list) = $ S' A"
-apply (induct_tac "A")
-apply (simp (no_asm))
+lemma scheme_list_substitutions_only_on_free_variables [rule_format]:
+  "(!x:free_tv A. (S x) = (S' x)) --> $ S (A::type_scheme list) = $ S' A"
+apply (induct_tac A)
+apply simp
 apply simp
 apply (rule weaken_asm_Un)
 apply (intro strip)
 apply (erule scheme_substitutions_only_on_free_variables)
 done
 
-lemma eq_subst_te_eq_free [rule_format (no_asm)]: 
-  "$ S1 (t::typ) = $ S2 t --> n:(free_tv t) --> S1 n = S2 n"
-apply (induct_tac "t")
-(* case TVar n *)
-apply (fastsimp)
-(* case Fun t1 t2 *)
-apply (fastsimp)
-done
+lemma eq_subst_te_eq_free:
+  "$ S1 (t::typ) = $ S2 t \<Longrightarrow> n:(free_tv t) \<Longrightarrow> S1 n = S2 n"
+  by (induct t) auto
 
-lemma eq_subst_type_scheme_eq_free [rule_format (no_asm)]: 
+lemma eq_subst_type_scheme_eq_free [rule_format]: 
   "$ S1 (sch::type_scheme) = $ S2 sch --> n:(free_tv sch) --> S1 n = S2 n"
 apply (induct_tac "sch")
 (* case TVar n *)
-apply (simp (no_asm_simp))
+apply simp
 (* case BVar n *)
 apply (intro strip)
 apply (erule mk_scheme_injective)
-apply (simp (no_asm_simp))
+apply simp
 (* case Fun t1 t2 *)
 apply simp
 done
 
-lemma eq_subst_scheme_list_eq_free [rule_format (no_asm)]: 
-  "$S1 (A::type_scheme list) = $S2 A --> n:(free_tv A) --> S1 n = S2 n"
-apply (induct_tac "A")
-(* case [] *)
-apply (fastsimp)
-(* case x#xl *)
-apply (fastsimp intro: eq_subst_type_scheme_eq_free)
-done
+lemma eq_subst_scheme_list_eq_free:
+  "$S1 (A::type_scheme list) = $S2 A \<Longrightarrow> n:(free_tv A) \<Longrightarrow> S1 n = S2 n"
+proof (induct A)
+  case Nil
+  then show ?case by fastsimp
+next
+  case Cons
+  then show ?case by (fastsimp intro: eq_subst_type_scheme_eq_free)
+qed
 
-lemma codD: 
-      "v : cod S ==> v : free_tv S"
-apply (unfold free_tv_subst)
-apply (fast)
-done
- 
-lemma not_free_impl_id: 
-      "x ~: free_tv S ==> S x = TVar x"
- 
-apply (unfold free_tv_subst dom_def)
-apply (fast)
-done
+lemma codD: "v : cod S ==> v : free_tv S"
+  unfolding free_tv_subst by blast
 
-lemma free_tv_le_new_tv: 
-      "[| new_tv n t; m:free_tv t |] ==> m<n"
-apply (unfold new_tv_def)
-apply (fast)
-done
+lemma not_free_impl_id: "x ~: free_tv S ==> S x = TVar x"
+  unfolding free_tv_subst dom_def by blast
 
-lemma cod_app_subst: 
+lemma free_tv_le_new_tv: "[| new_tv n t; m:free_tv t |] ==> m<n"
+  unfolding new_tv_def by blast
+
+lemma cod_app_subst [simp]:
   "[| v : free_tv(S n); v~=n |] ==> v : cod S"
 apply (unfold dom_def cod_def UNION_def Bex_def)
 apply (simp (no_asm))
@@ -441,119 +391,90 @@ apply (safe intro!: exI conjI notI)
 prefer 2 apply (assumption)
 apply simp
 done
-declare cod_app_subst [simp]
 
 lemma free_tv_subst_var: "free_tv (S (v::nat)) <= insert v (cod S)"
-apply (case_tac "v:dom S")
+apply (cases "v:dom S")
 apply (fastsimp simp add: cod_def)
 apply (fastsimp simp add: dom_def)
 done
 
 lemma free_tv_app_subst_te: "free_tv ($ S (t::typ)) <= cod S Un free_tv t"
-apply (induct_tac "t")
-(* case TVar n *)
-apply (simp (no_asm) add: free_tv_subst_var)
-(* case Fun t1 t2 *)
-apply (fastsimp)
-done
+proof (induct t)
+  case (TVar n) then show ?case by (simp add: free_tv_subst_var)
+next
+  case (Fun t1 t2) then show ?case by fastsimp
+qed
 
-lemma free_tv_app_subst_type_scheme: "free_tv ($ S (sch::type_scheme)) <= cod S Un free_tv sch"
-apply (induct_tac "sch")
-(* case FVar n *)
-apply (simp (no_asm) add: free_tv_subst_var)
-(* case BVar n *)
-apply (simp (no_asm))
-(* case Fun t1 t2 *)
-apply (fastsimp)
-done
+lemma free_tv_app_subst_type_scheme:
+    "free_tv ($ S (sch::type_scheme)) <= cod S Un free_tv sch"
+proof (induct sch)
+  case (FVar n)
+  then show ?case by (simp add: free_tv_subst_var)
+next
+  case (BVar n)
+  then show ?case by simp
+next
+  case (SFun t1 t2)
+  then show ?case by fastsimp
+qed
 
 lemma free_tv_app_subst_scheme_list: "free_tv ($ S (A::type_scheme list)) <= cod S Un free_tv A"
-apply (induct_tac "A")
-(* case [] *)
-apply (simp (no_asm))
-(* case a#al *)
-apply (cut_tac free_tv_app_subst_type_scheme)
-apply (fastsimp)
-done
+proof (induct A)
+  case Nil then show ?case by simp
+next
+  case (Cons a al)
+  with free_tv_app_subst_type_scheme
+  show ?case by fastsimp
+qed
 
 lemma free_tv_comp_subst: 
-     "free_tv (%u::nat. $ s1 (s2 u) :: typ) <=    
-      free_tv s1 Un free_tv s2"
-apply (unfold free_tv_subst dom_def)
-apply (force simp add: cod_def dom_def
-             dest!:free_tv_app_subst_te [THEN subsetD])
-done
+  "free_tv (%u::nat. $ s1 (s2 u) :: typ) <=    
+    free_tv s1 Un free_tv s2"
+  unfolding free_tv_subst dom_def
+  by (force simp add: cod_def dom_def
+    dest!:free_tv_app_subst_te [THEN subsetD])
 
 lemma free_tv_o_subst: 
-     "free_tv ($ S1 o S2) <= free_tv S1 Un free_tv (S2 :: nat => typ)"
-apply (unfold o_def)
-apply (rule free_tv_comp_subst)
-done
+    "free_tv ($ S1 o S2) <= free_tv S1 Un free_tv (S2 :: nat => typ)"
+  unfolding o_def by (rule free_tv_comp_subst)
 
-lemma free_tv_of_substitutions_extend_to_types [rule_format (no_asm)]: 
-  "n : free_tv t --> free_tv (S n) <= free_tv ($ S t::typ)"
-apply (induct_tac "t")
-apply (simp (no_asm))
-apply (simp (no_asm))
-apply fast
-done
+lemma free_tv_of_substitutions_extend_to_types:
+    "n : free_tv t \<Longrightarrow> free_tv (S n) <= free_tv ($ S t::typ)"
+  by (induct t) auto
 
-lemma free_tv_of_substitutions_extend_to_schemes [rule_format (no_asm)]: 
-  "n : free_tv sch --> free_tv (S n) <= free_tv ($ S sch::type_scheme)"
-apply (induct_tac "sch")
-apply (simp (no_asm))
-apply (simp (no_asm))
-apply (simp (no_asm))
-apply fast
-done
+lemma free_tv_of_substitutions_extend_to_schemes:
+    "n : free_tv sch \<Longrightarrow> free_tv (S n) <= free_tv ($ S sch::type_scheme)"
+  by (induct sch) auto
 
-lemma free_tv_of_substitutions_extend_to_scheme_lists [rule_format (no_asm)]: 
-  "n : free_tv A --> free_tv (S n) <= free_tv ($ S A::type_scheme list)"
-apply (induct_tac "A")
-apply (simp (no_asm))
-apply (simp (no_asm))
-apply (fast dest: free_tv_of_substitutions_extend_to_schemes)
-done
+lemma free_tv_of_substitutions_extend_to_scheme_lists [simp]:
+    "n : free_tv A \<Longrightarrow> free_tv (S n) <= free_tv ($ S A::type_scheme list)"
+  by (induct A) (auto dest: free_tv_of_substitutions_extend_to_schemes)
 
-declare free_tv_of_substitutions_extend_to_scheme_lists [simp]
+lemma free_tv_ML_scheme:
+  fixes sch :: type_scheme
+  shows "(n : free_tv sch) = (n: set (free_tv_ML sch))"
+  by (induct sch) simp_all
 
-lemma free_tv_ML_scheme: "!!sch::type_scheme. (n : free_tv sch) = (n: set (free_tv_ML sch))"
-apply (induct_tac "sch")
-apply (simp_all (no_asm_simp))
-done
-
-lemma free_tv_ML_scheme_list: "!!A::type_scheme list. (n : free_tv A) = (n: set (free_tv_ML A))"
-apply (induct_tac "A")
-apply (simp (no_asm))
-apply (simp (no_asm_simp) add: free_tv_ML_scheme)
-done
+lemma free_tv_ML_scheme_list:
+  fixes A :: "type_scheme list"
+  shows "(n : free_tv A) = (n: set (free_tv_ML A))"
+  by (induct_tac A) (simp_all add: free_tv_ML_scheme)
 
 
 -- "lemmata for @{text bound_tv}"
 
-lemma bound_tv_mk_scheme: "bound_tv (mk_scheme t) = {}"
-apply (induct_tac "t")
-apply (simp_all (no_asm_simp))
-done
+lemma bound_tv_mk_scheme [simp]: "bound_tv (mk_scheme t) = {}"
+  by (induct t) simp_all
 
-declare bound_tv_mk_scheme [simp]
+lemma bound_tv_subst_scheme [simp]:
+  fixes sch :: type_scheme
+  shows "bound_tv ($ S sch) = bound_tv sch"
+  by (induct sch) simp_all
 
-lemma bound_tv_subst_scheme: 
-  "!!sch::type_scheme. bound_tv ($ S sch) = bound_tv sch"
-apply (induct_tac "sch")
-apply (simp_all (no_asm_simp))
-done
-
-declare bound_tv_subst_scheme [simp]
-
-lemma bound_tv_subst_scheme_list: 
-  "!!A::type_scheme list. bound_tv ($ S A) = bound_tv A"
-apply (rule list.induct)
-apply (simp (no_asm))
-apply (simp (no_asm_simp))
-done
-
-declare bound_tv_subst_scheme_list [simp]
+lemma bound_tv_subst_scheme_list [simp]: 
+  fixes A :: "type_scheme list"
+  shows "bound_tv ($ S A) = bound_tv A"
+  by (induct A) simp_all
 
 
 -- "lemmata for @{text new_tv}"
@@ -579,31 +500,21 @@ apply (metis not_leE)+
 done
 
 lemma new_tv_list: "new_tv n x = (!y:set x. new_tv n y)"
-apply (induct_tac "x")
-apply (simp_all (no_asm_simp))
-done
+  by (induct x) simp_all
 
 -- "substitution affects only variables occurring freely"
-lemma subst_te_new_tv: 
-  "new_tv n (t::typ) --> $(%x. if x=n then t' else S x) t = $S t"
-apply (induct_tac "t")
-apply (simp_all (no_asm_simp))
-done
-declare subst_te_new_tv [simp]
+lemma subst_te_new_tv [simp]:
+    "new_tv n (t::typ) --> $(%x. if x=n then t' else S x) t = $S t"
+  by (induct t) simp_all
 
-lemma subst_te_new_type_scheme [rule_format (no_asm)]: 
-  "new_tv n (sch::type_scheme) --> $(%x. if x=n then sch' else S x) sch = $S sch"
-apply (induct_tac "sch")
-apply (simp_all (no_asm_simp))
-done
-declare subst_te_new_type_scheme [simp]
+lemma subst_te_new_type_scheme [simp]:
+    "new_tv n (sch::type_scheme) \<Longrightarrow> $(%x. if x=n then sch' else S x) sch = $S sch"
+  by (induct sch) simp_all
 
-lemma subst_tel_new_scheme_list [rule_format (no_asm)]: 
-  "new_tv n (A::type_scheme list) --> $(%x. if x=n then t else S x) A = $S A"
-apply (induct_tac "A")
-apply simp_all
-done
-declare subst_tel_new_scheme_list [simp]
+lemma subst_tel_new_scheme_list [simp]:
+    "new_tv n (A::type_scheme list) \<Longrightarrow> $(%x. if x=n then t else S x) A = $S A"
+  by (induct A) simp_all
+
 
 -- "all greater variables are also new"
 lemma new_tv_le: 
@@ -614,34 +525,29 @@ apply (drule spec)
 apply (erule (1) notE impE)
 apply (simp (no_asm))
 done
-declare lessI [THEN less_imp_le [THEN new_tv_le], simp]
+
+lemma [simp]: "new_tv n t \<Longrightarrow> new_tv (Suc n) t"
+  by (rule lessI [THEN less_imp_le [THEN new_tv_le]])
 
 lemma new_tv_typ_le: "n<=m ==> new_tv n (t::typ) ==> new_tv m t"
-apply (simp (no_asm_simp) add: new_tv_le)
-done
+  by (simp add: new_tv_le)
 
 lemma new_scheme_list_le: "n<=m ==> new_tv n (A::type_scheme list) ==> new_tv m A"
-apply (simp (no_asm_simp) add: new_tv_le)
-done
+  by (simp add: new_tv_le)
 
 lemma new_tv_subst_le: "n<=m ==> new_tv n (S::subst) ==> new_tv m S"
-apply (simp (no_asm_simp) add: new_tv_le)
-done
+  by (simp add: new_tv_le)
 
 -- "@{text new_tv} property remains if a substitution is applied"
 lemma new_tv_subst_var: 
   "[| n<m; new_tv m (S::subst) |] ==> new_tv m (S n)"
-apply (simp add: new_tv_subst)
-done
+  by (simp add: new_tv_subst)
 
-lemma new_tv_subst_te [rule_format (no_asm)]: 
-  "new_tv n S --> new_tv n (t::typ) --> new_tv n ($ S t)"
-apply (induct_tac "t")
-apply (fastsimp simp add: new_tv_subst)+
-done
-declare new_tv_subst_te [simp]
+lemma new_tv_subst_te [simp]:
+    "new_tv n S \<Longrightarrow> new_tv n (t::typ) \<Longrightarrow> new_tv n ($ S t)"
+  by (induct t) (auto simp add: new_tv_subst)
 
-lemma new_tv_subst_type_scheme [rule_format (no_asm)]: 
+lemma new_tv_subst_type_scheme [rule_format, simp]: 
   "new_tv n S --> new_tv n (sch::type_scheme) --> new_tv n ($ S sch)"
 apply (induct_tac "sch")
 apply (simp_all)
@@ -653,32 +559,25 @@ apply simp
 apply (drule_tac x = "m" in spec)
 apply fast
 done
-declare new_tv_subst_type_scheme [simp]
 
-lemma new_tv_subst_scheme_list [rule_format (no_asm)]: 
-  "new_tv n S --> new_tv n (A::type_scheme list) --> new_tv n ($ S A)"
-apply (induct_tac "A")
-apply (fastsimp)+
-done
-declare new_tv_subst_scheme_list [simp]
+lemma new_tv_subst_scheme_list [simp]:
+    "new_tv n S \<Longrightarrow> new_tv n (A::type_scheme list) \<Longrightarrow> new_tv n ($ S A)"
+  by (induct A) auto
 
 lemma new_tv_Suc_list: "new_tv n A --> new_tv (Suc n) ((TVar n)#A)"
-apply (simp (no_asm) add: new_tv_list)
-done
+  by (simp add: new_tv_list)
 
-lemma new_tv_only_depends_on_free_tv_type_scheme [rule_format (no_asm)]: 
-  "!!sch::type_scheme. (free_tv sch) = (free_tv sch') --> (new_tv n sch --> new_tv n sch')"
-apply (unfold new_tv_def)
-apply (simp (no_asm_simp))
-done
+lemma new_tv_only_depends_on_free_tv_type_scheme:
+  fixes sch :: type_scheme
+  shows "free_tv sch = free_tv sch' \<Longrightarrow> new_tv n sch \<Longrightarrow> new_tv n sch'"
+  unfolding new_tv_def by simp
 
-lemma new_tv_only_depends_on_free_tv_scheme_list [rule_format (no_asm)]: 
-  "!!A::type_scheme list. (free_tv A) = (free_tv A') --> (new_tv n A --> new_tv n A')"
-apply (unfold new_tv_def)
-apply (simp (no_asm_simp))
-done
+lemma new_tv_only_depends_on_free_tv_scheme_list:
+  fixes A :: "type_scheme list"
+  shows "free_tv A = free_tv A' \<Longrightarrow> new_tv n A \<Longrightarrow> new_tv n A'"
+  unfolding new_tv_def by simp
 
-lemma new_tv_nth_nat_A [rule_format (no_asm)]: 
+lemma new_tv_nth_nat_A [rule_format]: 
   "!nat. nat < length A --> new_tv n A --> (new_tv n (A!nat))"
 apply (unfold new_tv_def)
 apply (induct_tac "A")
@@ -692,25 +591,20 @@ done
 
 
 -- "composition of substitutions preserves @{text new_tv} proposition"
-lemma new_tv_subst_comp_1: 
+lemma new_tv_subst_comp_1 [simp]: 
   "[| new_tv n (S::subst); new_tv n R |] ==> new_tv n (($ R) o S)"
-apply (simp add: new_tv_subst)
-done
+  by (simp add: new_tv_subst)
 
-lemma new_tv_subst_comp_2: 
+lemma new_tv_subst_comp_2 [simp]:
   "[| new_tv n (S::subst); new_tv n R |] ==> new_tv n (%v.$ R (S v))"
-apply (simp add: new_tv_subst)
-done
-
-declare new_tv_subst_comp_1 [simp] new_tv_subst_comp_2 [simp]
+  by (simp add: new_tv_subst)
 
 -- "new type variables do not occur freely in a type structure"
-lemma new_tv_not_free_tv: 
-      "new_tv n A ==> n~:(free_tv A)"
-by (auto simp add: new_tv_def)
-declare new_tv_not_free_tv [simp]
+lemma new_tv_not_free_tv [simp]:
+    "new_tv n A ==> n~:(free_tv A)"
+  by (auto simp add: new_tv_def)
 
-lemma fresh_variable_types: "!!t::typ. ? n. (new_tv n t)"
+lemma fresh_variable_types [simp]: "!!t::typ. ? n. (new_tv n t)"
 apply (unfold new_tv_def)
 apply (induct_tac "t")
 apply (rule_tac x = "Suc nat" in exI)
@@ -718,13 +612,10 @@ apply (simp (no_asm_simp))
 apply (erule exE)+
 apply (rename_tac "n'")
 apply (rule_tac x = "max n n'" in exI)
-apply (simp (no_asm) add: less_max_iff_disj)
-apply blast
+apply (simp add: less_max_iff_disj)
 done
 
-declare fresh_variable_types [simp]
-
-lemma fresh_variable_type_schemes: 
+lemma fresh_variable_type_schemes [simp]:
   "!!sch::type_scheme. ? n. (new_tv n sch)"
 apply (unfold new_tv_def)
 apply (induct_tac "sch")
@@ -735,13 +626,10 @@ apply (simp (no_asm))
 apply (erule exE)+
 apply (rename_tac "n'")
 apply (rule_tac x = "max n n'" in exI)
-apply (simp (no_asm) add: less_max_iff_disj)
-apply blast
+apply (simp add: less_max_iff_disj)
 done
 
-declare fresh_variable_type_schemes [simp]
-
-lemma fresh_variable_type_scheme_lists: 
+lemma fresh_variable_type_scheme_lists [simp]: 
   "!!A::type_scheme list. ? n. (new_tv n A)"
 apply (induct_tac "A")
 apply (simp (no_asm))
@@ -754,10 +642,8 @@ apply (rule_tac x = " (max n n') " in exI)
 apply (subgoal_tac "n <= (max n n') ")
 apply (subgoal_tac "n' <= (max n n') ")
 apply (fast dest: new_tv_le)
-apply (simp_all (no_asm) add: le_max_iff_disj)
+apply (simp_all add: le_max_iff_disj)
 done
-
-declare fresh_variable_type_scheme_lists [simp]
 
 lemma make_one_new_out_of_two: 
   "[| ? n1. (new_tv n1 x); ? n2. (new_tv n2 y)|] ==> ? n. (new_tv n x) & (new_tv n y)"
@@ -802,115 +688,92 @@ done
 
 (* lemmata for substitutions *)
 
-lemma length_app_subst_list: 
+lemma length_app_subst_list [simp]:
    "!!A:: ('a::type_struct) list. length ($ S A) = length A"
+  unfolding app_subst_list by simp
 
-apply (unfold app_subst_list)
-apply (simp (no_asm))
-done
-declare length_app_subst_list [simp]
+lemma subst_TVar_scheme [simp]:
+  fixes sch :: type_scheme
+  shows "$ TVar sch = sch"
+  by (induct sch) simp_all
 
-lemma subst_TVar_scheme: "!!sch::type_scheme. $ TVar sch = sch"
-apply (induct_tac "sch")
-apply (simp_all (no_asm_simp))
-done
-
-declare subst_TVar_scheme [simp]
-
-lemma subst_TVar_scheme_list: "!!A::type_scheme list. $ TVar A = A"
-apply (rule list.induct)
-apply (simp_all add: app_subst_list)
-done
-
-declare subst_TVar_scheme_list [simp]
+lemma subst_TVar_scheme_list [simp]:
+  fixes A :: "type_scheme list"
+  shows "$ TVar A = A"
+  by (induct A) (simp_all add: app_subst_list)
 
 -- "application of @{text id_subst} does not change type expression"
-lemma app_subst_id_te: 
-  "$ id_subst = (%t::typ. t)"
+lemma app_subst_id_te [simp]: "$ id_subst = (%t::typ. t)"
 apply (unfold id_subst_def)
 apply (rule ext)
 apply (induct_tac "t")
-apply (simp_all (no_asm_simp))
+apply simp_all
 done
-declare app_subst_id_te [simp]
 
-lemma app_subst_id_type_scheme: 
+lemma app_subst_id_type_scheme [simp]:
   "$ id_subst = (%sch::type_scheme. sch)"
 apply (unfold id_subst_def)
 apply (rule ext)
 apply (induct_tac "sch")
-apply (simp_all (no_asm_simp))
+apply simp_all
 done
-declare app_subst_id_type_scheme [simp]
 
 -- "application of @{text id_subst} does not change list of type expressions"
-lemma app_subst_id_tel: 
+lemma app_subst_id_tel [simp]: 
   "$ id_subst = (%A::type_scheme list. A)"
 apply (unfold app_subst_list)
 apply (rule ext)
 apply (induct_tac "A")
-apply (simp_all (no_asm_simp))
-done
-declare app_subst_id_tel [simp]
-
-lemma id_subst_sch: "!!sch::type_scheme. $ id_subst sch = sch"
-apply (induct_tac "sch")
-apply (simp_all add: id_subst_def)
-done
-
-declare id_subst_sch [simp]
-
-lemma id_subst_A: "!!A::type_scheme list. $ id_subst A = A"
-apply (induct_tac "A")
-apply simp
-apply simp
-done
-
-declare id_subst_A [simp]
-
--- "composition of substitutions"
-lemma o_id_subst: "$S o id_subst = S"
-apply (unfold id_subst_def o_def)
-apply (rule ext)
-apply (simp (no_asm))
-done
-declare o_id_subst [simp]
-
-lemma subst_comp_te: "$ R ($ S t::typ) = $ (%x. $ R (S x) ) t"
-apply (induct_tac "t")
-apply (simp_all (no_asm_simp))
-done
-
-lemma subst_comp_type_scheme: 
-  "$ R ($ S sch::type_scheme) = $ (%x. $ R (S x) ) sch"
-apply (induct_tac "sch")
 apply simp_all
 done
 
+lemma id_subst_sch [simp]:
+  fixes sch :: type_scheme
+  shows "$ id_subst sch = sch"
+  by (induct sch) (simp_all add: id_subst_def)
+
+lemma id_subst_A [simp]:
+  fixes A :: "type_scheme list"
+  shows "$ id_subst A = A"
+  by (induct A) simp_all
+
+-- "composition of substitutions"
+lemma o_id_subst [simp]: "$S o id_subst = S"
+  unfolding id_subst_def o_def by simp
+
+lemma subst_comp_te: "$ R ($ S t::typ) = $ (%x. $ R (S x) ) t"
+  by (induct t) simp_all
+
+lemma subst_comp_type_scheme: 
+  "$ R ($ S sch::type_scheme) = $ (%x. $ R (S x) ) sch"
+  by (induct sch) simp_all
+
 lemma subst_comp_scheme_list: 
   "$ R ($ S A::type_scheme list) = $ (%x. $ R (S x)) A"
-apply (unfold app_subst_list)
-apply (induct_tac "A")
-(* case [] *)
-apply (simp (no_asm))
-(* case x#xl *)
-apply (simp add: subst_comp_type_scheme)
-done
+unfolding app_subst_list
+proof (induct A)
+  case Nil then show ?case by simp
+next
+  case (Cons x xl)
+  then show ?case by (simp add: subst_comp_type_scheme)
+qed
 
 lemma subst_id_on_type_scheme_list': 
-  "!!A::type_scheme list. !x : free_tv A. S x = (TVar x) ==> $ S A = $ id_subst A"
+  fixes A :: "type_scheme list"
+  shows "!x : free_tv A. S x = (TVar x) ==> $ S A = $ id_subst A"
 apply (rule scheme_list_substitutions_only_on_free_variables)
 apply (simp add: id_subst_def)
 done
 
 lemma subst_id_on_type_scheme_list: 
-  "!!A::type_scheme list. !x : free_tv A. S x = (TVar x) ==> $ S A = A"
+  fixes A :: "type_scheme list"
+  shows "!x : free_tv A. S x = (TVar x) ==> $ S A = A"
 apply (subst subst_id_on_type_scheme_list')
 apply assumption
-apply (simp (no_asm))
+apply simp
 done
 
-lemma nth_subst [rule_format (no_asm)]: 
+lemma nth_subst [rule_format]: 
   "!n. n < length A --> ($ S A)!n = $S (A!n)"
 apply (induct_tac "A")
 apply simp
